src/single_auth_message/DY.Example.SingleAuthMessage.Protocol.Stateful.fst
@@ -1,16 +1,16 @@
-module DY.Example.SingleConfMessage.Protocol.Stateful
+module DY.Example.SingleAuthMessage.Protocol.Stateful
 
 open Comparse
 open DY.Core
 open DY.Lib
-open DY.Example.SingleConfMessage.Protocol.Total
+open DY.Example.SingleAuthMessage.Protocol.Total
 
 (*** State type ***)
 
 [@@with_bytes bytes]
 type single_message_state =
-  | SenderState: receiver:principal -> secret:bytes -> single_message_state
-  | ReceiverState: secret:bytes -> payload:bytes -> single_message_state
+  | SenderState: sender:principal -> secret:bytes -> single_message_state
+  | ReceiverState: sender:principal -> secret:bytes -> payload:bytes -> single_message_state
 
 %splice [ps_single_message_state] (gen_parser (`single_message_state))
 %splice [ps_single_message_state_is_well_formed] (gen_is_well_formed_lemma (`single_message_state))
@@ -19,7 +19,7 @@ instance parseable_serializeable_bytes_single_message_state: parseable_serialize
  = mk_parseable_serializeable ps_single_message_state
 
 instance local_state_single_message_state: local_state single_message_state = {
-  tag = "SingleConfMessage.State";
+  tag = "SingleAuthMessage.State";
   format = parseable_serializeable_bytes_single_message_state;
 }
 
@@ -27,14 +27,14 @@ instance local_state_single_message_state: local_state single_message_state = {
 
 [@@with_bytes bytes]
 type single_message_event =
-  | SenderSendMsg: sender:principal -> receiver:principal -> secret:bytes -> single_message_event
+  | SenderSendMsg: sender:principal -> secret:bytes -> single_message_event
   | ReceiverReceivedMsg: sender:principal -> receiver:principal -> secret:bytes -> payload:bytes -> single_message_event
 
 %splice [ps_single_message_event] (gen_parser (`single_message_event))
 %splice [ps_single_message_event_is_well_formed] (gen_is_well_formed_lemma (`single_message_event))
 
-instance event_single_message_event: event single_message_event = {
-  tag = "SingleConfMessage.Event";
+instance event_protocol_event: event single_message_event = {
+  tag = "SingleAuthMessage.Event";
   format = mk_parseable_serializeable ps_single_message_event;
 }
 
@@ -42,28 +42,29 @@ instance event_single_message_event: event single_message_event = {
 
 val prepare_message: principal -> principal -> traceful state_id
 let prepare_message sender receiver =
-  let* secret = mk_rand NoUsage (join (principal_label sender) (principal_label receiver)) 32 in
+  let* secret = mk_rand NoUsage public 32 in
+  trigger_event sender (SenderSendMsg sender secret);*
   let* state_id = new_session_id sender in
-  set_state sender state_id (SenderState receiver secret <: single_message_state);*
+  set_state sender state_id (SenderState sender secret <: single_message_state);*
   return state_id
 
 val send_message: communication_keys_sess_ids -> principal -> principal -> state_id -> traceful (option timestamp)
 let send_message comm_keys_ids sender receiver state_id =
   let*? st:single_message_state = get_state sender state_id in
   match st with
-  | SenderState receiver secret -> (
+  | SenderState sender secret -> (
     let msg = compute_message secret in
-    trigger_event sender (SenderSendMsg sender receiver secret);*
-    let*? msg_id = send_confidential comm_keys_ids sender receiver msg in
+    trigger_event sender (SenderSendMsg sender secret);*
+    let*? msg_id = send_authenticated comm_keys_ids sender receiver msg in
     return (Some msg_id)
   )
   | _ -> return None
 
 val receive_message: communication_keys_sess_ids -> principal -> timestamp -> traceful (option state_id)
 let receive_message comm_keys_ids receiver msg_id =
-  let*? msg:communication_message_base = receive_confidential comm_keys_ids receiver msg_id in
+  let*? msg:communication_message_base = receive_authenticated comm_keys_ids receiver msg_id in
   let*? single_msg:single_message = return (decode_message msg.payload) in
   trigger_event receiver (ReceiverReceivedMsg msg.sender receiver single_msg.secret msg.payload);*
   let* state_id = new_session_id receiver in
-  set_state receiver state_id (ReceiverState single_msg.secret msg.payload <: single_message_state);*
+  set_state receiver state_id (ReceiverState msg.sender single_msg.secret msg.payload <: single_message_state);*
   return (Some state_id)
