src/single_auth_message/DY.Example.SingleAuthMessage.Protocol.Total.Proof.fst
@@ -1,0 +1,118 @@
+module DY.Example.SingleAuthMessage.Protocol.Total.Proof
+
+open Comparse
+open DY.Core
+open DY.Lib
+open DY.Example.SingleAuthMessage.Protocol.Total
+open DY.Example.SingleAuthMessage.Protocol.Stateful
+
+#set-options "--fuel 0 --ifuel 0 --z3cliopt 'smt.qi.eager_threshold=100'"
+
+(*** Cryptographic invariants ***)
+
+val crypto_usages_protocol: crypto_usages
+instance crypto_usages_protocol = default_crypto_usages
+
+val pkenc_pred_list_protocol: list (string & pkenc_crypto_predicate crypto_usages_protocol)
+let pkenc_pred_list_protocol = [
+  pkenc_crypto_predicates_communication_layer_and_tag
+]
+
+val sign_pred_list_protocol: list (string & sign_crypto_predicate crypto_usages_protocol)
+let sign_pred_list_protocol = [
+  sign_crypto_predicates_communication_layer_and_tag;
+]
+
+#push-options "--ifuel 2 --fuel 0"
+val crypto_predicates_protocol: crypto_predicates crypto_usages_protocol
+let crypto_predicates_protocol = {
+  default_crypto_predicates crypto_usages_protocol with
+
+  pkenc_pred = mk_pkenc_predicate pkenc_pred_list_protocol;
+
+  sign_pred = mk_sign_predicate sign_pred_list_protocol;
+}
+
+instance crypto_invariants_protocol: crypto_invariants = {
+  usages = crypto_usages_protocol;
+  preds = crypto_predicates_protocol;
+}
+#pop-options
+
+#push-options "--ifuel 0 --fuel 1"
+val pkenc_pred_has_all_pkenc_preds: 
+  unit ->
+  Lemma
+  (ensures
+    norm [delta_only [`%pkenc_pred_list_protocol; `%for_allP]; iota; zeta] (
+      for_allP (has_pkenc_predicate crypto_invariants_protocol) pkenc_pred_list_protocol
+    )
+  )
+let pkenc_pred_has_all_pkenc_preds () =
+  assert_norm(List.Tot.no_repeats_p (List.Tot.map fst (pkenc_pred_list_protocol)));
+  mk_pkenc_predicate_correct crypto_invariants_protocol pkenc_pred_list_protocol;
+  norm_spec [delta_only [`%pkenc_pred_list_protocol; `%for_allP]; iota; zeta] (for_allP (has_pkenc_predicate crypto_invariants_protocol) pkenc_pred_list_protocol);
+  ()
+
+val sign_pred_has_all_sign_preds:
+  unit ->
+  Lemma
+  (ensures
+    norm [delta_only [`%sign_pred_list_protocol; `%for_allP]; iota; zeta] (
+      for_allP (has_sign_predicate crypto_invariants_protocol) sign_pred_list_protocol
+    )
+  )
+let sign_pred_has_all_sign_preds () =
+  assert_norm(List.Tot.no_repeats_p (List.Tot.map fst (sign_pred_list_protocol)));
+  mk_sign_predicate_correct crypto_invariants_protocol sign_pred_list_protocol;
+  norm_spec [delta_only [`%sign_pred_list_protocol; `%for_allP]; iota; zeta] (for_allP (has_sign_predicate crypto_invariants_protocol) sign_pred_list_protocol);
+  ()
+#pop-options
+
+val protocol_crypto_invariants_has_communication_layer_invariants: squash (has_communication_layer_invariants crypto_invariants_protocol)
+let protocol_crypto_invariants_has_communication_layer_invariants =
+  pkenc_pred_has_all_pkenc_preds ();
+  sign_pred_has_all_sign_preds ();
+  ()
+
+(*** Proofs ***)
+
+val compute_message_proof:
+  tr:trace ->
+  sender:principal -> receiver:principal ->
+  secret:bytes ->
+  Lemma
+  (requires
+    event_triggered tr sender (SenderSendMsg sender secret) /\
+    is_publishable tr secret
+  )
+  (ensures
+    is_publishable tr (compute_message secret)
+  )
+let compute_message_proof tr sender receiver secret =
+  serialize_wf_lemma single_message (is_publishable tr) {secret;};
+  ()
+
+val decode_message_proof:
+  tr:trace ->
+  sender:principal -> receiver:principal ->
+  msg_bytes:bytes ->
+  Lemma
+  (requires
+    is_publishable tr msg_bytes
+  )
+  (ensures (
+    match decode_message msg_bytes with
+    | Some msg -> (
+      is_publishable tr msg.secret
+    )
+    | None -> True
+  )
+  )
+let decode_message_proof tr sender receiver msg_bytes =
+  match decode_message msg_bytes with
+  | Some msg -> (
+    parse_wf_lemma single_message (is_publishable tr) msg_bytes;
+    ()
+  )
+  | None -> ()
