src/single_auth_message/DY.Example.SingleAuthMessage.SecurityProperties.fst
@@ -1,0 +1,25 @@
+module DY.Example.SingleAuthMessage.SecurityProperties
+
+open Comparse
+open DY.Core
+open DY.Lib
+open DY.Example.SingleAuthMessage.Protocol.Total
+open DY.Example.SingleAuthMessage.Protocol.Total.Proof
+open DY.Example.SingleAuthMessage.Protocol.Stateful
+open DY.Example.SingleAuthMessage.Protocol.Stateful.Proof
+
+#set-options "--fuel 0 --ifuel 0 --z3rlimit 10  --z3cliopt 'smt.qi.eager_threshold=100'"
+
+val sender_authentication:
+  tr:trace -> sender:principal -> receiver:principal -> secret:bytes ->
+  Lemma
+  (requires
+    trace_invariant tr /\
+    event_triggered tr receiver (ReceiverReceivedMsg sender receiver secret (compute_message secret))
+  )
+  (ensures
+    event_triggered tr sender (SenderSendMsg sender secret) \/
+    (exists vk_sender. event_triggered tr receiver (CommAuthReceiveMsg sender receiver vk_sender (compute_message secret)) /\
+      is_corrupt tr (get_signkey_label vk_sender))
+  )
+let sender_authentication tr sender receiver secret = ()
