Makefile
@@ -1,5 +1,5 @@
 DY_HOME ?= ../../..
 
-EXAMPLES = single_conf_message
+EXAMPLES = single_conf_message single_auth_message
 EXAMPLE_DIRS = $(addprefix src/, $(EXAMPLES))
 include $(DY_HOME)/Makefile
